dataplane/Examples/Increment_top.thy
@@ -72,17 +72,17 @@ abbreviation inp_incr_edges where
   \<open>inp_incr_edges \<equiv> (\<lambda>l. if l = Loc (0 :: 2) (Src (0 :: 1)) then [Loc (1 :: 2) (Trg (0 :: 1))] else [])\<close>
 
 abbreviation inp_incr_summary where
-  \<open>inp_incr_summary \<equiv> (\<lambda>l1 l2.
+  \<open>inp_incr_summary incr \<equiv> (\<lambda>l1 l2.
   if l1 = Loc (0 :: 2) (Src (0 :: 1)) \<and> l2 = Loc (1 :: 2) (Trg (0 :: 1))
   then antichain {0}
   else if l1 = Loc 0 (Trg 0) \<and> l2 = Loc 0 (Src 0)
-  then antichain {0}
+  then antichain {incr 0}
   else if l1 = Loc 1 (Trg 0) \<and> l2 = Loc 1 (Src 0)
   then antichain {0}
   else {}\<^sub>A)\<close>
 
 lemma
-  \<open>summ sg = inp_incr_summary \<Longrightarrow>
+  \<open>summ sg = inp_incr_summary incr \<Longrightarrow>
   \<forall>x \<in> set (buf (Inr (1, 0))). is_Inr x \<Longrightarrow>
   dataflow_op sg (inp_incr_op os1 caps ins buf incr os2)
   \<approx> map_op (\<lambda>(p :: 1). (1, p)) (\<lambda>p. (1, p))
